src/examples/durable_stack.v
@@ -12,7 +12,7 @@ From self.high Require Import dprop.
 From self.lang Require Import notation lang.
 From self.algebra Require Import view.
 From self.base Require Import primitive_laws class_instances.
-From self.high Require Import proofmode wpc_proofmode.
+From self.high Require Import proofmode wpc_proofmode or_lost.
 From self.high Require Import dprop abstract_state_instances modalities
      resources crash_weakestpre weakestpre weakestpre_na weakestpre_at
      recovery_weakestpre lifted_modalities protocol no_buffer.
@@ -22,14 +22,14 @@ From self.high.modalities Require Import fence.
 
 (* A node is a pointer to a value and a pointer to the next node. *)
 (* NOTE: The [mk_node] function is currently unused. *)
-Definition mk_node : expr :=
-  λ: "v" "next",
-    let: "val" := ref_NA "v" in
-    let: "toNext" := ref_NA "next" in
-    ref_NA (InjR ("val", "toNext")).
+(* Definition mk_node : expr := *)
+(*   λ: "v" "next", *)
+(*     let: "val" := ref_NA "v" in *)
+(*     let: "toNext" := ref_NA "next" in *)
+(*     ref_NA (InjR ("val", "toNext")). *)
 
-Definition mk_nil : expr :=
-  λ: <>, ref_NA (InjL #()).
+(* Definition mk_nil : expr := *)
+(*   λ: <>, ref_NA (InjL #()). *)
 
 Definition mk_stack : expr :=
   λ: <>,
@@ -74,36 +74,33 @@ Section constant_prot.
   Context `{Σ : gFunctors}.
   Context `{nvmFixedG Σ}.
 
-  Definition constant_prot `{nvmFixedG Σ} (v1 : val) (_ : unit) (v2 : val)
-             (hG : nvmDeltaG Σ) : dProp Σ :=
-    ⌜ v1 = v2 ⌝.
-
-  Global Program Instance constant_prot_prot v :
-    LocationProtocol (constant_prot v) := { bumper n := n }.
+  Program Definition constant_prot v1 : LocationProtocol unit :=
+    {| pred := λ _ v2 _, ⌜ v1 = v2 ⌝%I;
+       bumper v := v |}.
   Next Obligation. iIntros. by iApply post_crash_flush_pure. Qed.
 
 End constant_prot.
 
 Definition mapsto_na_flushed `{nvmFixedG Σ, nvmDeltaG Σ, AbstractState ST}
-           ℓ q (s : ST) : dProp Σ :=
-  ∃ p (ss : list ST),
+           ℓ (prot : LocationProtocol ST) q (s : ST) : dProp Σ :=
+  ∃ (ss : list ST),
     "%lastEq" ∷ ⌜ last ss = Some s ⌝ ∗
-    "pts" ∷ ℓ ↦_{p}^{q} ss ∗
-    "#flushLb" ∷ know_flush_lb ℓ s.
+    "pts" ∷ ℓ ↦_{prot}^{q} ss ∗
+    "#flushLb" ∷ know_flush_lb ℓ prot s.
 
 Section mapsto_na_flushed.
   Context `{nvmFixedG Σ, nvmDeltaG Σ, AbstractState ST}.
 
-  Global Instance buffer_free_mapsto_na_flushed ℓ q (s : ST) :
-    BufferFree (mapsto_na_flushed ℓ q s).
+  Global Instance buffer_free_mapsto_na_flushed ℓ prot q (s : ST) :
+    BufferFree (mapsto_na_flushed ℓ prot q s).
   Proof. apply _. Qed.
 
-  Lemma mapsto_na_flushed_agree ℓ q q' (s s' : ST) :
-    mapsto_na_flushed ℓ q s -∗ mapsto_na_flushed ℓ q' s' -∗ ⌜ s = s' ⌝.
+  Lemma mapsto_na_flushed_agree ℓ prot q q' (s s' : ST) :
+    mapsto_na_flushed ℓ prot q s -∗ mapsto_na_flushed ℓ prot q' s' -∗ ⌜ s = s' ⌝.
   Proof.
     rewrite /mapsto_na_flushed.
     iNamed 1.
-    iDestruct 1 as (? ss' last') "[pts' lb']".
+    iDestruct 1 as (ss' last') "[pts' lb']".
     rewrite /mapsto_na. iNamed "pts".
     iDestruct "pts'" as (?????) "(? & ? & ? & %look & %nolater' & ? & ? & ? & ? & ? & ? & ?)".
     iDestruct (ghost_map_elem_agree with "hist [$]") as %<-%(inj _).
@@ -116,16 +113,16 @@ Section mapsto_na_flushed.
     - eexists _. rewrite look. done.
   Qed.
 
-  Lemma mapsto_na_flushed_split ℓ p q (s : ST) :
-    mapsto_na_flushed ℓ (p + q) s -∗
-    mapsto_na_flushed ℓ p s ∗ mapsto_na_flushed ℓ q s.
+  Lemma mapsto_na_flushed_split ℓ prot p q (s : ST) :
+    mapsto_na_flushed ℓ prot (p + q) s -∗
+    mapsto_na_flushed ℓ prot p s ∗ mapsto_na_flushed ℓ prot q s.
   Proof.
-    iDestruct 1 as (? ss last) "[[pts1 pts2] #flushLb]".
-    iSplitL "pts1"; iFrame "flushLb"; iExists _, ss; iFrame (last) "∗".
+    iDestruct 1 as (ss last) "[[pts1 pts2] #flushLb]".
+    iSplitL "pts1"; iFrame "flushLb"; iExists ss; iFrame (last) "∗".
   Qed.
 
-  Global Instance mapsto_na_flushed_fractional ℓ (s : ST) :
-    Fractional (λ q, mapsto_na_flushed ℓ q s).
+  Global Instance mapsto_na_flushed_fractional ℓ prot (s : ST) :
+    Fractional (λ q, mapsto_na_flushed ℓ prot q s).
   Proof.
     rewrite /Fractional.
     intros p q.
@@ -133,7 +130,7 @@ Section mapsto_na_flushed.
     - iApply mapsto_na_flushed_split.
     - iIntros "[L R]".
       iNamed "R".
-      iDestruct "L" as (???) "[[pts1' pts2'] _]".
+      iDestruct "L" as (??) "[[pts1' pts2'] _]".
       (* This direction is more annoying to show (not impossible) *)
   Abort.
 
@@ -146,9 +143,9 @@ Section mapsto_na_flushed.
   (* Proof. *)
   (*   Admitted. *)
 
-  Global Instance mapsto_na_flushed_post_crash_flushed ℓ q (s : ST) :
-    IntoCrashFlush (mapsto_na_flushed ℓ q s)
-                   (λ _, mapsto_na_flushed ℓ q s ∗ recovered_at ℓ s)%I.
+  Global Instance mapsto_na_flushed_post_crash_flushed ℓ prot q (s : ST) :
+    IntoCrashFlush (mapsto_na_flushed ℓ prot q s)
+                   (λ _, mapsto_na_flushed ℓ prot q s ∗ recovered_at ℓ s)%I.
   Proof.
     rewrite /IntoCrashFlush.
     iNamed 1.
@@ -160,7 +157,7 @@ Section mapsto_na_flushed.
     iDestruct (post_crash_mapsto_na with "pts") as "pts".
     iDestruct (post_crash_flush_post_crash with "pts") as "pts".
     iCrashFlush.
-    iDestruct "flushLb" as (s' ?) "(#r & ? & ? & ?)".
+    iDestruct "flushLb" as (s' ?) "(#r & ?)".
     iDestruct (recovered_at_or_lost with "r pts") as "(%s'' & ? & pts & ?)".
     iDestruct (recovered_at_agree with "r [$]") as %<-.
     (* We can't prove that with this approach, but it is (will be) true. *)
@@ -195,46 +192,54 @@ Section definitions.
        changed.
    *)
 
-  Definition toNext_prot : loc_pred (singl val) :=
-    λ '(mk_singl v) v' _, ⌜ v = v' ⌝%I.
+  Program Definition toNext_prot : LocationProtocol (singl val) :=
+    {| pred := λ '(mk_singl v) v' _, ⌜ v = v' ⌝%I;
+       bumper v := v |}.
+  Next Obligation. iIntros (?[?]?) "H". iCrashFlush. done. Qed.
+  Next Obligation. destruct s. simpl. apply _. Qed.
+  
+  (* Definition toNext_prot : loc_pred (singl val) := *)
+  (*   λ '(mk_singl v) v' _, ⌜ v = v' ⌝%I. *)
 
   Definition nil_node_prot := constant_prot (InjLV #()).
 
-  Definition cons_node_prot (x : val) (ℓtoNext : loc) : loc_pred unit :=
-    λ (_ : unit) (v : val) (hG : nvmDeltaG Σ),
-      (⌜ v = InjRV (x, #ℓtoNext)%V ⌝)%I.
+  Definition cons_node_prot (x : val) (ℓtoNext : loc) :=
+    constant_prot (InjRV (x, #ℓtoNext)).
+
+    (* λ (_ : unit) (v : val) (hG : nvmDeltaG Σ), *)
+    (*   (⌜ v = InjRV (x, #ℓtoNext)%V ⌝)%I. *)
     (* ∗ ϕ x hG)%I. *)
 
-  Program Instance toNext_prot_prot :
-    LocationProtocol toNext_prot := { bumper n := n }.
-  Next Obligation. iIntros (?[?]?) "H". iCrashFlush. done. Qed.
-  Next Obligation. destruct s. apply _. Qed.
+  (* Program Instance toNext_prot_prot : *)
+  (*   LocationProtocol toNext_prot := { bumper n := n }. *)
+  (* Next Obligation. iIntros (?[?]?) "H". iCrashFlush. done. Qed. *)
+  (* Next Obligation. destruct s. apply _. Qed. *)
 
-  Program Instance cons_node_prot_prot x ℓ :
-    LocationProtocol (cons_node_prot x ℓ) := { bumper n := n }.
-  Next Obligation.
-    iIntros (?????).
-    rewrite /cons_node_prot.
-    iIntros "?".
-    (* iDestruct 1 as "[A B]". *)
-    iCrashFlush. naive_solver.
-  Qed.
+  (* Program Instance cons_node_prot_prot x ℓ : *)
+  (*   LocationProtocol (cons_node_prot x ℓ) := { bumper n := n }. *)
+  (* Next Obligation. *)
+  (*   iIntros (?????). *)
+  (*   rewrite /cons_node_prot. *)
+  (*   iIntros "?". *)
+  (*   (* iDestruct 1 as "[A B]". *) *)
+  (*   iCrashFlush. naive_solver. *)
+  (* Qed. *)
 
   (* Representation predicate for a node. *)
   Fixpoint is_node `{nvmDeltaG Σ} ℓnode (xs : list val) : dProp Σ :=
     match xs with
-    | [] => ∃ q p,
-        ℓnode ↦_{p}^{q} [()] ∗
-        know_protocol ℓnode nil_node_prot ∗
-        know_flush_lb ℓnode ()
-    | x :: xs' => ∃ (ℓtoNext ℓnext : loc) p1 q1 q2,
+    | [] => ∃ q,
+        ℓnode ↦_{nil_node_prot}^{q} [()] ∗
+        (* know_protocol ℓnode nil_node_prot ∗ *)
+        know_flush_lb ℓnode nil_node_prot ()
+    | x :: xs' => ∃ (ℓtoNext ℓnext : loc) q1 q2,
         (* ℓnode *)
-        ℓnode ↦_{p1}^{q1} [()] ∗
-        know_protocol ℓnode (cons_node_prot x ℓtoNext) ∗
-        know_flush_lb ℓnode () ∗
+        ℓnode ↦_{cons_node_prot x ℓtoNext}^{q1} [()] ∗
+        (* know_protocol ℓnode (cons_node_prot x ℓtoNext) ∗ *)
+        know_flush_lb ℓnode (cons_node_prot x ℓtoNext) () ∗
         (* ℓtoNext *)
-        know_protocol ℓtoNext toNext_prot ∗
-        mapsto_na_flushed ℓtoNext q2 (mk_singl #ℓnext) ∗
+        (* know_protocol ℓtoNext toNext_prot ∗ *)
+        mapsto_na_flushed ℓtoNext toNext_prot q2 (mk_singl #ℓnext) ∗
         (* know_protocol ℓnext (constant_prot #ℓnode) ∗ *)
         is_node ℓnext xs'
     end.
@@ -252,24 +257,24 @@ Section definitions.
     rewrite /IntoCrashFlush.
     generalize dependent ℓnode.
     induction xs as [|x xs IH]; iIntros (ℓnode).
-    - iDestruct 1 as (??) "(nodePts & prot & lb)".
+    - iDestruct 1 as (?) "(nodePts & lb)".
       iCrashFlush.
-      iDestruct "lb" as ([] le) "(#rec & ? & lb & ?)".
+      iDestruct "lb" as ([] le) "(#rec & lb)".
       iDestruct (recovered_at_or_lost with "rec nodePts") as "nodePts".
-      iDestruct (recovered_at_or_lost with "rec prot") as "prot".
       iDestruct "nodePts" as ([] elem) "(nodePts & ?)".
-      iExists _, _. iFrame "nodePts". iFrame.
-    - iDestruct 1 as (?????) "(nodePts & nodeProt & nodeFlushLb &
-                               toNextProt & toNextFlush & node)".
+      iExists _. iFrame "nodePts". iFrame.
+      iApply persist_lb_to_flush_lb.
+      iFrame "lb".
+    - iDestruct 1 as (????) "(nodePts & nodeFlushLb & toNextFlush & node)".
       iApply IH in "node".
       iCrashFlush.
-      iDestruct "nodeFlushLb" as ([]?) "(#nodeRec & ? & toNextFlushLb & ?)" .
+      iDestruct "nodeFlushLb" as ([] ?) "(#nodeRec & toNextFlushLb)" .
       iDestruct "toNextFlush" as "[toNextFlush toNextRec]".
-      iDestruct (recovered_at_or_lost with "toNextRec toNextProt") as "toNextProt".
-      iDestruct (recovered_at_or_lost with "nodeRec nodeProt") as "nodeProt".
       iDestruct (recovered_at_or_lost with "nodeRec nodePts") as "nodePts".
       iDestruct "nodePts" as ([]?) "[nodePts _]".
-      iExists _, _, _, _, q2.
+      iExists _, _, _, q2.
+      iFrame.
+      iApply persist_lb_to_flush_lb.
       iFrame.
   Qed.
 
@@ -278,9 +283,9 @@ Section definitions.
   Proof.
     generalize dependent ℓnode.
     induction xs as [|x xs IH]; iIntros (ℓnode).
-    - iDestruct 1 as (q?) "([pts1 pts2] & #r)".
+    - iDestruct 1 as (q) "([pts1 pts2] & #r)".
       iSplitL "pts1"; iFrame "r"; naive_solver.
-    - iDestruct 1 as (?????) "([pts1 pts2] & #? & #? & #? & toNextPts & node)".
+    - iDestruct 1 as (????) "([pts1 pts2] & #? & toNextPts & node)".
       rewrite -(Qp_div_2 q2).
       iDestruct (mapsto_na_flushed_split with "toNextPts") as "[toNextPts1 toNextPts2]".
       iDestruct (IH with "node") as "[node1 node2]".
@@ -291,18 +296,16 @@ Section definitions.
 
   (* The invariant for the location that points to the first node in the
   stack. *)
-  Definition toHead_prot `{nvmDeltaG Σ} (_ : unit) (v : val) (hG : nvmDeltaG Σ) : dProp Σ :=
-    ∃ (ℓnode : loc) xs,
-      "%vEqNode" ∷ ⌜ v = #ℓnode ⌝ ∗
-      "isNode" ∷ is_node ℓnode xs ∗
-      "#phis" ∷ ([∗ list] x ∈ xs, ϕ x _).
-      (* "#nodeFlushLb" ∷ know_flush_lb ℓnode (). *)
-
-  Program Instance stack_inv_prot `{nvmDeltaG Σ} :
-    LocationProtocol (toHead_prot) := { bumper n := n }.
+  Program Definition toHead_prot `{nvmDeltaG Σ} :=
+    {| pred (_ : unit) (v : val) _ :=
+        (∃ (ℓnode : loc) xs,
+          "%vEqNode" ∷ ⌜ v = #ℓnode ⌝ ∗
+          "isNode" ∷ is_node ℓnode xs ∗
+          "#phis" ∷ ([∗ list] x ∈ xs, ϕ x _))%I;
+      bumper s := s;
+    |}.
   Next Obligation.
     iIntros (????).
-    rewrite /toHead_prot.
     iNamed 1.
     iCrashFlush.
     iExists ℓnode, _.
@@ -313,9 +316,8 @@ Section definitions.
   Definition is_stack `{nvmDeltaG Σ} (v : val) : dProp Σ :=
     ∃ (ℓtoHead : loc),
       ⌜ v = #ℓtoHead ⌝ ∗
-      know_protocol ℓtoHead toHead_prot ∗
       ⎡ is_at_loc ℓtoHead ⎤ ∗
-      know_store_lb ℓtoHead ().
+      know_store_lb ℓtoHead toHead_prot ().
 
 End definitions.
 
@@ -335,14 +337,15 @@ Section proof.
   Proof.
     rewrite /is_stack.
     iDestruct 1 as (? [= <-]) "prot".
-    iDestruct "prot" as "(a & b & c)".
+    iDestruct "prot" as "(a & c)".
     iDestruct (post_crash_know_store_lb with "c")  as "c".
     iCrash.
-    iCombine "a b c" as "a".
-    rewrite 2!or_lost_sep.
+    iCombine "a c" as "a".
+    rewrite !or_lost_sep.
     iApply (or_lost_mono with "[] a").
-    iIntros "(a & b & (%u & c))". destruct u. iExists _. iSplitPure; first done.
+    iIntros "(a & (%u & c))". destruct u. iExists _. iSplitPure; first done.
     iFrame.
+    iApply persist_lb_to_store_lb. iFrame.
   Qed.
 
   Lemma wp_mk_stack :
@@ -354,7 +357,7 @@ Section proof.
     rewrite /mk_stack.
     wp_pures.
     wp_apply (wp_alloc_na _ () nil_node_prot with "[//]").
-    iIntros (ℓnil) "[#nilProt nilPts]".
+    iIntros (ℓnil) "nilPts".
     iDestruct (mapsto_na_store_lb with "nilPts") as "#storeLb"; first done.
     wp_pures.
     wp_apply (wp_wb_lb with "[$]").
@@ -368,8 +371,8 @@ Section proof.
       iExists _, [].
       iSplitPure; first reflexivity.
       simpl. iFrame "#".
-      iExists _, _. iFrame. }
-    iNext. iIntros (?) "(hi & ho & hip)".
+      iExists _. iFrame. }
+    iNext. iIntros (?) "(? & ?)".
     iApply "ϕpost".
     iExists _. naive_solver.
   Qed.
@@ -380,20 +383,21 @@ Section proof.
     {{{ RET #(); True }}}.
   Proof.
     iIntros (Φ)
-      "[#(%ℓstack & -> & #(stackProt & stackSh & stackLb)) #phi] ϕpost".
+      "[#(%ℓstack & -> & #(stackSh & stackLb)) #phi] ϕpost".
     rewrite /push.
     wp_pures.
-    wp_apply (wp_alloc_na _ (mk_singl _) toNext_prot with "[//]").
-    iIntros (ℓtoNext) "[#toNextProt toNextPts]".
+    wp_apply (wp_alloc_na _ (mk_singl _) toNext_prot with "[]").
+    { simpl. done. }
+    iIntros (ℓtoNext) "toNextPts".
     wp_pures.
     wp_apply (wp_alloc_na _ () (cons_node_prot x ℓtoNext)).
     { done. } (* rewrite /cons_node_prot. iFrame. done. } *)
-    iIntros (ℓnode) "[#nodeProt nodePts]".
+    iIntros (ℓnode) "nodePts".
     wp_pures.
     wp_apply (wp_wb_ex with "nodePts"); first reflexivity.
     iIntros "[nodePts #nodeFlushLb]".
     wp_pure1. wp_pure1. wp_pure1.
-    iAssert (∃ xs x', ⌜ last xs = Some x' ⌝ ∗ ℓtoNext ↦_{false} xs)%I with "[toNextPts]" as "toNextPts".
+    iAssert (∃ xs x', ⌜ last xs = Some x' ⌝ ∗ ℓtoNext ↦_{_} xs)%I with "[toNextPts]" as "toNextPts".
     { iExists _, _. iFrame. done. }
     iLöb as "IH".
     iDestruct "toNextPts" as (xs' x' lastEq) "toNextPts".
@@ -401,7 +405,7 @@ Section proof.
 
     (* The load of the pointer to the head. *)
     wp_apply (wp_load_at _ _ (λ _ v, (∃ (ℓhead : loc) xs, ⌜v = #ℓhead⌝ ∗ is_node ℓhead xs ∗ _)%I) with "[]").
-    { iFrame "stackProt stackSh stackLb".
+    { iFrame "stackSh stackLb".
       iModIntro.
       iIntros ([] v le) "toHead".
       iNamed "toHead".
@@ -415,7 +419,7 @@ Section proof.
     wp_pures.
     wp_apply (wp_store_na _ _ _ _ _ (mk_singl v) with "[$toNextPts]").
     { done. } { done. }
-    { iFrame "toNextProt". done. }
+    { simpl. done. }
     simpl.
     iIntros "toNextPts".
     wp_pures.
@@ -427,7 +431,7 @@ Section proof.
     wp_pures.
 
     wp_apply (wp_cas_at (λ _, True)%I (λ _, True)%I with "[nodePts toNextPts isNode]").
-    { iFrame "stackProt stackSh stackLb".
+    { iFrame "stackSh stackLb".
       iSplit.
       { iIntros (??).
         iSplitL "".
@@ -442,10 +446,8 @@ Section proof.
         (* iFrame "nodeFlushLb". *)
         iExists _, _ , _, _.
         iFrame "isNode".
-        iFrame "nodeProt".
-        iFrame "toNextProt".
         iFrame "nodePts nodeFlushLb".
-        iExists _, _, _. iFrame "toNextPts toNextPtsFl".
+        iExists _. iFrame "toNextPts toNextPtsFl".
         iPureIntro. apply last_app. done. }
       iIntros (??).
       iSplitL ""; first iIntros "!> $ //". iAccu. }
@@ -465,14 +467,14 @@ Section proof.
     {{{ v, RET v;
         (⌜ v = NONEV ⌝) ∨ (∃ x, ⌜ v = InjRV x ⌝ ∗ ϕ x _) }}}.
   Proof.
-    iIntros (Φ) "#(%ℓstack & -> & #(stackProt & stackSh & stackLb)) ϕpost".
+    iIntros (Φ) "#(%ℓstack & -> & #(stackSh & stackLb)) ϕpost".
     rewrite /pop.
     wp_pure1.
     iLöb as "IH".
     wp_pures.
     wp_apply (wp_load_at _ _
          (λ _ v, (∃ (ℓhead : loc) xs, ⌜v = #ℓhead⌝ ∗ is_node ℓhead xs ∗ _)%I) with "[]").
-    { iFrame "stackProt stackSh stackLb".
+    { iFrame "stackSh stackLb".
       iModIntro.
       iIntros ([] v le) "toHead".
       iNamed "toHead".
@@ -488,8 +490,8 @@ Section proof.
     wp_pures.
     destruct xs as [|x xs]; simpl.
     - (* The queue is empty. *)
-      iDestruct "node" as (??) "(headPts & #headProt & #headLb)".
-      wp_apply (wp_load_na with "[$headPts $headProt]").
+      iDestruct "node" as (?) "(headPts & #headLb)".
+      wp_apply (wp_load_na with "[$headPts]").
       { done. }
       { iModIntro. iIntros (?). rewrite /constant_prot. iIntros "#eq".
         iFrame "eq". iDestruct "eq" as "-#eq". rewrite right_id. iAccu. }
@@ -499,17 +501,16 @@ Section proof.
       iApply "ϕpost". iLeft. done.
     - (* The queue is non-empty. *)
       iDestruct "phis" as "[phi phis]".
-      iDestruct "node" as (?????)
-        "(headPts & #headProt & #headFlushLb & #toNextProt & toNextPts & node)".
-      wp_apply (wp_load_na with "[$headPts $headProt]").
+      iDestruct "node" as (????) "(headPts & #headFlushLb & toNextPts & node)".
+      wp_apply (wp_load_na with "[$headPts]").
       { done. }
       { iModIntro. iIntros (?) "#eq". iFrame "eq". iDestruct "eq" as "-#eq". 
         rewrite right_id. iAccu. }
       simpl.
-      iIntros (v) "[headPts ->]".
+      iIntros (v) "[headPts <-]".
       wp_pures.
       iNamed "toNextPts".
-      wp_apply (wp_load_na with "[$pts $toNextProt]").
+      wp_apply (wp_load_na with "[$pts]").
       { done. }
       { iModIntro. iIntros (?). rewrite /toNext_prot. iIntros "#eq".
         iFrame "eq". iDestruct "eq" as "-#eq". rewrite right_id. iAccu. }
@@ -518,7 +519,7 @@ Section proof.
       wp_pures.
 
       wp_apply (wp_cas_at (λ _, True)%I (λ _, True)%I with "[node]").
-      { iFrame "stackProt stackSh stackLb".
+      { iFrame "stackSh stackLb".
         iSplit.
         { iIntros (??).
           iSplitL "".
